src/PredCalc/MultiSubst.v
@@ -48,13 +48,13 @@ Section syntax.
     | _ => af
     end.
 
-  Definition var_term_map_fvars m : gset variable :=
+  Definition vtmap_fvars m : gset variable :=
     ⋃ (term_fvars ∘ snd <$> map_to_list m).
 
-  Lemma elem_of_var_term_map_fvars x m :
-    x ∈ var_term_map_fvars m → ∃ y t, m !! y = Some t ∧ x ∈ term_fvars t.
+  Lemma elem_of_vtmap_fvars x m :
+    x ∈ vtmap_fvars m → ∃ y t, m !! y = Some t ∧ x ∈ term_fvars t.
   Proof with auto.
-    intros. unfold var_term_map_fvars in H. apply elem_of_union_list in H as [fvars []].
+    intros. unfold vtmap_fvars in H. apply elem_of_union_list in H as [fvars []].
     induction m using map_ind.
     - rewrite map_to_list_empty in H. simpl in H. apply elem_of_nil in H as [].
     - rewrite map_to_list_insert in H... simpl in H.
@@ -65,10 +65,10 @@ Section syntax.
         discriminate.
   Qed.
 
-  Lemma not_elem_of_var_term_map_fvars x m :
-    x ∉ var_term_map_fvars m → (∀ y t, m !! y = Some t → x ∉ term_fvars t).
+  Lemma not_elem_of_vtmap_fvars x m :
+    x ∉ vtmap_fvars m → (∀ y t, m !! y = Some t → x ∉ term_fvars t).
   Proof with auto.
-    intros. unfold var_term_map_fvars in H. unfold not in H. intros contra.
+    intros. unfold vtmap_fvars in H. unfold not in H. intros contra.
     apply H. clear H. apply elem_of_union_list. exists (term_fvars t). split...
     induction m using map_ind.
     - apply lookup_empty_Some in H0 as [].
@@ -78,7 +78,7 @@ Section syntax.
   Qed.
 
   Definition quant_msubst_fvars y A m :=
-    (formula_fvars A ∖ {[y]}) ∪ var_term_map_fvars m ∪ dom m.
+    (formula_fvars A ∖ {[y]}) ∪ vtmap_fvars m ∪ dom m.
 
   Lemma quant_msubst_fvars_inv y' y A m :
     y' ∉ quant_msubst_fvars y A m →
@@ -87,7 +87,7 @@ Section syntax.
     intros. unfold quant_msubst_fvars in H. do 2 rewrite not_elem_of_union in H.
     destruct_and! H. split_and!...
     - apply not_elem_of_difference in H. set_solver.
-    - apply not_elem_of_var_term_map_fvars...
+    - apply not_elem_of_vtmap_fvars...
   Qed.
 
   Equations? msubst A m : formula by wf (rank A) lt :=
@@ -108,15 +108,15 @@ Section syntax.
     deduce_rank_eq H. rewrite Hfr. rewrite Hqr. lia.
   Qed.
 
-  Definition to_var_term_map (xs : list variable) (ts : list term)
-    `{OfSameLength variable term xs ts}: gmap variable term := list_to_map (zip xs ts).
+  Definition to_vtmap (xs : list variable) (ts : list term)
+    `{!OfSameLength xs ts}: gmap variable term := list_to_map (zip xs ts).
 
-  Local Notation "t [ [ₜ xs \ ts ] ]" := (msubst_term t (to_var_term_map xs ts))
+  Local Notation "t [ [ₜ xs \ ts ] ]" := (msubst_term t (to_vtmap xs ts))
                                            (in custom formula at level 74, left associativity,
                                                xs custom var_seq,
                                                ts custom term_seq) : refiney_scope.
 
-  Local Notation "A [ [ xs \ ts ] ]" := (msubst A (to_var_term_map xs ts))
+  Local Notation "A [ [ xs \ ts ] ]" := (msubst A (to_vtmap xs ts))
                                           (in custom formula at level 74, left associativity,
                                               xs custom var_seq,
                                               ts custom term_seq) : refiney_scope.
@@ -195,13 +195,13 @@ Section syntax.
   (* TODO: can I replace all teval equiv lemmas with simple equality? Or at least tequiv? *)
   Lemma msubst_term_non_free t xs ts `{!OfSameLength xs ts} :
     list_to_set xs ## term_fvars t →
-    msubst_term t (to_var_term_map xs ts) = t.
+    msubst_term t (to_vtmap xs ts) = t.
   Proof with auto.
     intros. induction t; simpl...
-    - destruct (to_var_term_map xs ts !! x) eqn:E.
-      + apply elem_of_dom_2 in E. unfold to_var_term_map in E.
+    - destruct (to_vtmap xs ts !! x) eqn:E.
+      + apply elem_of_dom_2 in E. unfold to_vtmap in E.
         rewrite dom_list_to_map_zip_L in E... set_solver.
-      + apply not_elem_of_dom_2 in E. unfold to_var_term_map in E.
+      + apply not_elem_of_dom_2 in E. unfold to_vtmap in E.
         rewrite dom_list_to_map_zip_L in E...
     - f_equal. induction args... simpl. f_equal.
       + simpl in H0. apply H0... set_solver.
@@ -212,7 +212,7 @@ Section syntax.
 
   Lemma msubst_af_non_free af xs ts `{!OfSameLength xs ts} :
     list_to_set xs ## af_fvars af →
-    msubst_af af (to_var_term_map xs ts) = af.
+    msubst_af af (to_vtmap xs ts) = af.
   Proof with auto.
     intros. destruct af; simpl in *...
     - rewrite msubst_term_non_free by set_solver. rewrite msubst_term_non_free by set_solver...
@@ -223,11 +223,11 @@ Section syntax.
   Qed.
 
   Lemma fvars_msubst_term_superset t xs ts `{!OfSameLength xs ts} :
-    term_fvars (msubst_term t (to_var_term_map xs ts)) ⊆ term_fvars t ∪ ⋃ (term_fvars <$> ts).
+    term_fvars (msubst_term t (to_vtmap xs ts)) ⊆ term_fvars t ∪ ⋃ (term_fvars <$> ts).
   Proof with auto.
     induction t; simpl; [set_solver| | ].
-    - destruct (to_var_term_map xs ts !! x) eqn:E.
-      + unfold to_var_term_map in E. apply lookup_list_to_map_zip_Some in E as (i&?&?&_)...
+    - destruct (to_vtmap xs ts !! x) eqn:E.
+      + unfold to_vtmap in E. apply lookup_list_to_map_zip_Some in E as (i&?&?&_)...
         apply elem_of_list_lookup_2 in H0. set_unfold. intros x0 ?. right.
         apply elem_of_union_list. exists (term_fvars t). set_solver.
       + simpl. set_solver.
@@ -248,20 +248,20 @@ Section syntax.
     intros Hnodup ?. induction t; simpl; [set_solver | |].
     - destruct (decide (x ∈ xs)).
       + apply elem_of_list_lookup in e as (i&?). destruct (lookup_of_same_length_l ts H0) as (t&?).
-        * replace (to_var_term_map xs ts !! x) with (Some t).
+        * replace (to_vtmap xs ts !! x) with (Some t).
           -- intros x' ?. set_unfold. right. apply elem_of_union_list. exists (term_fvars t).
              split... apply elem_of_list_fmap. exists t. split...
              apply elem_of_list_lookup_2 in H1...
-          -- symmetry. unfold to_var_term_map. apply lookup_list_to_map_zip_Some...
+          -- symmetry. unfold to_vtmap. apply lookup_list_to_map_zip_Some...
              exists i. split_and!... intros. apply NoDup_lookup with (i:=i) in H2...
              lia.
-      + replace (to_var_term_map xs ts !! x) with (@None term); [set_solver|].
-        symmetry. unfold to_var_term_map. apply lookup_list_to_map_zip_None...
+      + replace (to_vtmap xs ts !! x) with (@None term); [set_solver|].
+        symmetry. unfold to_vtmap. apply lookup_list_to_map_zip_None...
     - induction args; simpl; [set_solver|]. set_solver.
   Qed.
 
   Lemma fvars_msubst_af_superset af xs ts `{!OfSameLength xs ts} :
-    af_fvars (msubst_af af (to_var_term_map xs ts)) ⊆ af_fvars af ∪ ⋃ (term_fvars <$> ts).
+    af_fvars (msubst_af af (to_vtmap xs ts)) ⊆ af_fvars af ∪ ⋃ (term_fvars <$> ts).
   Proof with auto.
     destruct af; simpl; [set_solver|set_solver | | |].
     - pose proof (fvars_msubst_term_superset t1 xs ts).
@@ -278,7 +278,7 @@ Section syntax.
     induction A; simp msubst; simpl.
     2-4: set_solver.
     - apply fvars_msubst_af_superset.
-    - generalize_fresh_var_for_msubst x A (to_var_term_map xs ts) as x'.
+    - generalize_fresh_var_for_msubst x A (to_vtmap xs ts) as x'.
       forward (H <! A [x \ x'] !>)... clear H2 H3 H4.
       destruct (decide (x ∈ formula_fvars A)).
       + rewrite fvars_subst_free in H... set_solver.
@@ -311,7 +311,7 @@ Section syntax.
       apply (final_term_final t) in H0...
   Qed.
 
-  Lemma msubst_term_trans t xs1 xs2 ts `{!OfSameLength xs1 xs2} `{!OfSameLength xs2 ts}
+  Lemma msubst_term_trans t xs1 xs2 ts `{!OfSameLength xs1 (⇑ₓ₊ xs2)} `{!OfSameLength xs2 ts}
       `{!OfSameLength xs1 ts} :
     xs1 ## xs2 →
     NoDup xs1 →
@@ -322,31 +322,32 @@ Section syntax.
     intros Hdisjoint Hnodup1 Hnodup2 Hfree. induction t...
     - simpl. destruct (decide (x ∈ xs1 ∨ x ∈ xs2)).
       2:{ apply Decidable.not_or in n as [].
-          simpl. replace (to_var_term_map xs1 (@TVar value <$> xs2) !! x) with (@None term).
-          2:{ symmetry. unfold to_var_term_map. apply lookup_list_to_map_zip_None...
-              typeclasses eauto. }
-          replace (to_var_term_map xs1 ts !! x) with (@None term).
-          2:{ symmetry. unfold to_var_term_map. apply lookup_list_to_map_zip_None... }
-          simpl. replace (to_var_term_map xs2 ts !! x) with (@None term)...
-          symmetry. unfold to_var_term_map. apply lookup_list_to_map_zip_None... }
+          simpl. replace (to_vtmap xs1 (@TVar value <$> xs2) !! x) with (@None term).
+          2:{ symmetry. unfold to_vtmap. apply lookup_list_to_map_zip_None... }
+          replace (to_vtmap xs1 ts !! x) with (@None term).
+          2:{ symmetry. unfold to_vtmap. apply lookup_list_to_map_zip_None... }
+          simpl. replace (to_vtmap xs2 ts !! x) with (@None term)...
+          symmetry. unfold to_vtmap. apply lookup_list_to_map_zip_None... }
       destruct o.
       + pose proof (Hdisjoint x H).
         apply elem_of_list_lookup in H as [i ?].
         destruct (lookup_of_same_length_l ts H) as [t ?].
+        assert (OfSameLength xs1 xs2).
+        { unfold OfSameLength in OfSameLength0. rewrite length_fmap in OfSameLength0... }
         destruct (lookup_of_same_length_l xs2 H) as [x' ?].
-        replace (to_var_term_map xs1 (@TVar value <$> xs2) !! x) with (Some (@TVar value x')).
-        2:{ symmetry. unfold to_var_term_map. apply lookup_list_to_map_zip_Some;
+        replace (to_vtmap xs1 (@TVar value <$> xs2) !! x) with (Some (@TVar value x')).
+        2:{ symmetry. unfold to_vtmap. apply lookup_list_to_map_zip_Some;
             [typeclasses eauto|]. exists i. split_and!...
             - apply list_lookup_fmap_Some. exists x'. split...
-            - intros. apply NoDup_lookup with (i:=i) in H3... lia. }
-        simpl. replace (to_var_term_map xs2 ts !! x') with (Some t).
-        2:{ symmetry. unfold to_var_term_map. apply lookup_list_to_map_zip_Some;
+            - intros. apply NoDup_lookup with (i:=i) in H4... lia. }
+        simpl. replace (to_vtmap xs2 ts !! x') with (Some t).
+        2:{ symmetry. unfold to_vtmap. apply lookup_list_to_map_zip_Some;
             [typeclasses eauto|]. exists i. split_and!...
-            intros. apply NoDup_lookup with (i:=i) in H3... lia. }
-        replace (to_var_term_map xs1 ts !! x) with (Some t)...
-        symmetry. unfold to_var_term_map. apply lookup_list_to_map_zip_Some;
+            intros. apply NoDup_lookup with (i:=i) in H4... lia. }
+        replace (to_vtmap xs1 ts !! x) with (Some t)...
+        symmetry. unfold to_vtmap. apply lookup_list_to_map_zip_Some;
           [typeclasses eauto|]. exists i. split_and!...
-        intros. apply NoDup_lookup with (i:=i) in H3... lia.
+        intros. apply NoDup_lookup with (i:=i) in H4... lia.
       + assert (x ∉ xs1) by (intros contra; apply (Hdisjoint x); auto).
         simpl in Hfree. set_unfold in Hfree. simpl in Hfree. apply Hfree in H as []...
     - simpl. f_equal. apply list_eq. rewrite <- list_fmap_compose. intros i.
@@ -365,38 +366,38 @@ Section syntax.
     intros Hdisjoint Hnodup1 Hnodup2 Hfree1 Hfree2. induction t...
     - simpl. destruct (decide (x ∈ xs1 ∨ x ∈ xs2)).
       2:{ apply Decidable.not_or in n as [].
-          simpl. replace (to_var_term_map (xs1 ++ xs2) (ts1 ++ ts2) !! x) with (@None term).
-          2:{ symmetry. unfold to_var_term_map. apply lookup_list_to_map_zip_None...
+          simpl. replace (to_vtmap (xs1 ++ xs2) (ts1 ++ ts2) !! x) with (@None term).
+          2:{ symmetry. unfold to_vtmap. apply lookup_list_to_map_zip_None...
               - typeclasses eauto.
               - set_solver. }
-          replace (to_var_term_map xs1 ts1 !! x) with (@None term).
-          2:{ symmetry. unfold to_var_term_map. apply lookup_list_to_map_zip_None... }
-          simpl. replace (to_var_term_map xs2 ts2 !! x) with (@None term)...
-          symmetry. unfold to_var_term_map. apply lookup_list_to_map_zip_None... }
+          replace (to_vtmap xs1 ts1 !! x) with (@None term).
+          2:{ symmetry. unfold to_vtmap. apply lookup_list_to_map_zip_None... }
+          simpl. replace (to_vtmap xs2 ts2 !! x) with (@None term)...
+          symmetry. unfold to_vtmap. apply lookup_list_to_map_zip_None... }
       destruct o.
       + pose proof (Hdisjoint x H).
         apply elem_of_list_lookup in H as [i ?].
         destruct (lookup_of_same_length_l ts1 H) as [t ?].
-        replace (to_var_term_map (xs1 ++ xs2) (ts1 ++ ts2) !! x) with (Some t).
-        2:{ symmetry. unfold to_var_term_map. apply lookup_list_to_map_zip_Some;
+        replace (to_vtmap (xs1 ++ xs2) (ts1 ++ ts2) !! x) with (Some t).
+        2:{ symmetry. unfold to_vtmap. apply lookup_list_to_map_zip_Some;
             [typeclasses eauto|]. exists i. split_and!...
             - rewrite lookup_app. rewrite H...
             - rewrite lookup_app. rewrite H1...
             - intros. apply lookup_app_l_Some_disjoint' in H2...
               apply NoDup_lookup with (i:=i) in H2... lia. }
-        simpl. replace (to_var_term_map xs1 ts1 !! x) with (Some t).
-        2:{ symmetry. unfold to_var_term_map. apply lookup_list_to_map_zip_Some;
+        simpl. replace (to_vtmap xs1 ts1 !! x) with (Some t).
+        2:{ symmetry. unfold to_vtmap. apply lookup_list_to_map_zip_Some;
             [typeclasses eauto|]. exists i. split_and!...
             intros. apply NoDup_lookup with (i:=i) in H2... lia. }
-        rewrite msubst_term_id... unfold to_var_term_map. rewrite dom_list_to_map_zip_L...
+        rewrite msubst_term_id... unfold to_vtmap. rewrite dom_list_to_map_zip_L...
         clear dependent x. intros x ??. apply (Hfree2 _ H). apply elem_of_union_list.
         exists (term_fvars t). split... apply elem_of_list_fmap. apply elem_of_list_lookup_2 in H1.
         exists t...
       + assert (x ∉ xs1) by (intros contra; apply (Hdisjoint x); auto).
         apply elem_of_list_lookup in H as [i ?].
         destruct (lookup_of_same_length_l ts2 H) as [t ?].
-        replace (to_var_term_map (xs1 ++ xs2) (ts1 ++ ts2) !! x) with (Some t).
-        2:{ symmetry. unfold to_var_term_map. apply lookup_list_to_map_zip_Some;
+        replace (to_vtmap (xs1 ++ xs2) (ts1 ++ ts2) !! x) with (Some t).
+        2:{ symmetry. unfold to_vtmap. apply lookup_list_to_map_zip_Some;
             [typeclasses eauto|]. exists (i + length xs1).
             opose proof (@of_same_length _ _ xs1 ts1 _)... split_and!...
             - rewrite lookup_app. replace (xs1 !! (i + length xs1)) with (@None variable).
@@ -408,11 +409,11 @@ Section syntax.
               rewrite Nat.add_sub. rewrite H1...
             - intros. apply lookup_app_r_Some_disjoint' in H3 as []...
               apply NoDup_lookup with (i:=i) in H4... subst. lia. }
-        replace (to_var_term_map xs1 ts1 !! x) with (@None term).
-        2:{ symmetry. unfold to_var_term_map. apply lookup_list_to_map_zip_None;
+        replace (to_vtmap xs1 ts1 !! x) with (@None term).
+        2:{ symmetry. unfold to_vtmap. apply lookup_list_to_map_zip_None;
             [typeclasses eauto|]... }
-        simpl. replace (to_var_term_map xs2 ts2 !! x) with (Some t)...
-        symmetry. unfold to_var_term_map. apply lookup_list_to_map_zip_Some; [typeclasses eauto|].
+        simpl. replace (to_vtmap xs2 ts2 !! x) with (Some t)...
+        symmetry. unfold to_vtmap. apply lookup_list_to_map_zip_Some; [typeclasses eauto|].
         exists i. split_and!... intros. apply NoDup_lookup with (i:=i) in H2... lia.
     - simpl. f_equal. apply list_eq. rewrite <- list_fmap_compose. intros i.
       f_equal. induction args... simpl. rewrite H; [| left; auto].
@@ -430,37 +431,37 @@ Section syntax.
     intros Hdisjoint Hnodup1 Hnodup2 Hfree1 Hfree2. induction t...
     - simpl. destruct (decide (x ∈ xs1 ∨ x ∈ xs2)).
       2:{ apply Decidable.not_or in n as [].
-          simpl. assert (to_var_term_map xs1 ts1 !! x = @None term).
-          { unfold to_var_term_map. apply lookup_list_to_map_zip_None... }
-          assert (to_var_term_map xs2 ts2 !! x = @None term).
-          { unfold to_var_term_map. apply lookup_list_to_map_zip_None... }
+          simpl. assert (to_vtmap xs1 ts1 !! x = @None term).
+          { unfold to_vtmap. apply lookup_list_to_map_zip_None... }
+          assert (to_vtmap xs2 ts2 !! x = @None term).
+          { unfold to_vtmap. apply lookup_list_to_map_zip_None... }
           rewrite H1. rewrite H2. simpl. rewrite H1. rewrite H2... }
       destruct o.
       + pose proof (Hdisjoint x H).
         apply elem_of_list_lookup in H as [i ?].
         destruct (lookup_of_same_length_l ts1 H) as [t ?].
-        assert (to_var_term_map xs1 ts1 !! x = Some t).
-        { unfold to_var_term_map. apply lookup_list_to_map_zip_Some;
+        assert (to_vtmap xs1 ts1 !! x = Some t).
+        { unfold to_vtmap. apply lookup_list_to_map_zip_Some;
             [typeclasses eauto|]. exists i. split_and!... intros.
             apply NoDup_lookup with (i:=i) in H2... lia. }
         rewrite H2. rewrite msubst_term_id.
-        2:{ unfold to_var_term_map. rewrite dom_list_to_map_zip_L...
+        2:{ unfold to_vtmap. rewrite dom_list_to_map_zip_L...
             clear dependent x. intros x ??. apply (Hfree2 _ H). apply elem_of_union_list.
             exists (term_fvars t). split... apply elem_of_list_fmap.
             apply elem_of_list_lookup_2 in H1. exists t... }
-        replace (to_var_term_map xs2 ts2 !! x) with (@None term).
-        2:{ symmetry. unfold to_var_term_map. apply lookup_list_to_map_zip_None... }
+        replace (to_vtmap xs2 ts2 !! x) with (@None term).
+        2:{ symmetry. unfold to_vtmap. apply lookup_list_to_map_zip_None... }
         simpl. rewrite H2...
       + assert (x ∉ xs1) by (intros contra; apply (Hdisjoint x); auto).
-        replace (to_var_term_map xs1 ts1 !! x) with (@None term).
-        2:{ symmetry. unfold to_var_term_map. apply lookup_list_to_map_zip_None... }
+        replace (to_vtmap xs1 ts1 !! x) with (@None term).
+        2:{ symmetry. unfold to_vtmap. apply lookup_list_to_map_zip_None... }
         apply elem_of_list_lookup in H as [i ?].
         destruct (lookup_of_same_length_l ts2 H) as [t ?].
-        simpl. replace (to_var_term_map xs2 ts2 !! x) with (Some t).
-        2:{ symmetry. unfold to_var_term_map. apply lookup_list_to_map_zip_Some;
+        simpl. replace (to_vtmap xs2 ts2 !! x) with (Some t).
+        2:{ symmetry. unfold to_vtmap. apply lookup_list_to_map_zip_Some;
             [typeclasses eauto|]. exists i. split_and!... intros.
             apply NoDup_lookup with (i:=i) in H2... lia. }
-        rewrite msubst_term_id... unfold to_var_term_map. rewrite dom_list_to_map_zip_L...
+        rewrite msubst_term_id... unfold to_vtmap. rewrite dom_list_to_map_zip_L...
         clear dependent x. intros x ??. apply (Hfree1 _ H). apply elem_of_union_list.
         exists (term_fvars t). split... apply elem_of_list_fmap.
         apply elem_of_list_lookup_2 in H1. exists t...
@@ -481,9 +482,9 @@ Section syntax.
     set_solver.
   Qed.
 
-  Lemma msubst_term_diag t xs :
+  Lemma msubst_term_diag' t xs :
     NoDup xs →
-    msubst_term t (list_to_map (zip xs (TVar <$> xs))) = t.
+    msubst_term t (list_to_map (zip  xs (TVar <$> xs))) = t.
   Proof with auto.
     intros Hnodup. induction t...
     - simpl. destruct (decide (x ∈ xs)).
@@ -499,13 +500,18 @@ Section syntax.
       simpl. rewrite H; [| left]... f_equal. apply IHargs. intros. apply H. right...
   Qed.
 
+  Lemma msubst_term_diag t xs `{!OfSameLength xs (@TVar value <$> xs)} :
+    NoDup xs →
+    msubst_term t (to_vtmap xs (TVar <$> xs)) = t.
+  Proof with auto. unfold to_vtmap. apply msubst_term_diag'... Qed.
+
 End syntax.
 
-Notation "t [ [ₜ xs \ ts ] ]" := (msubst_term t (to_var_term_map xs ts))
+Notation "t [ [ₜ xs \ ts ] ]" := (msubst_term t (to_vtmap xs ts))
                             (in custom formula at level 74, left associativity,
                               xs custom var_seq,
                               ts custom term_seq) : refiney_scope.
-Notation "A [ [ xs \ ts ] ]" := (msubst A (to_var_term_map xs ts))
+Notation "A [ [ xs \ ts ] ]" := (msubst A (to_vtmap xs ts))
                             (in custom formula at level 74, left associativity,
                               xs custom var_seq,
                               ts custom term_seq) : refiney_scope.
@@ -535,13 +541,13 @@ Section semantics.
   Implicit Types m : gmap variable term.
   Implicit Types mv : gmap variable value.
 
-  Definition teval_var_term_map σ m mv :=
+  Definition teval_vtmap σ m mv :=
       dom mv = dom m ∧ ∀ x t v, m !! x = Some t → mv !! x = Some v → teval σ t v.
 
-  Lemma teval_var_term_map_total σ m :
-    ∃ mv : gmap variable value, teval_var_term_map σ m mv.
+  Lemma teval_vtmap_total σ m :
+    ∃ mv : gmap variable value, teval_vtmap σ m mv.
   Proof with auto.
-    unfold teval_var_term_map. induction m using map_ind.
+    unfold teval_vtmap. induction m using map_ind.
     - exists ∅. split... intros. apply lookup_empty_Some in H. contradiction.
     - rename x into t. rename i into x. destruct (teval_total σ t) as [v Hv].
       destruct IHm as (mv&?&?). exists (<[x:=v]> mv). split.
@@ -553,11 +559,11 @@ Section semantics.
           apply (H1 x' t' v' H2 H3).
   Qed.
 
-  Lemma teval_var_term_map_insert {σ m mv} x t v :
+  Lemma teval_vtmap_insert {σ m mv} x t v :
     teval σ t v →
-    teval_var_term_map σ m mv → teval_var_term_map σ (<[x:=t]> m) (<[x:=v]> mv).
+    teval_vtmap σ m mv → teval_vtmap σ (<[x:=t]> m) (<[x:=v]> mv).
   Proof with auto.
-    intros ? []. unfold teval_var_term_map. split.
+    intros ? []. unfold teval_vtmap. split.
     - apply set_eq. intros. do 2 rewrite dom_insert. rewrite H0...
     - intros. destruct (decide (x = x0)).
       + subst. rewrite (lookup_insert mv) in H3. rewrite (lookup_insert m) in H2.
@@ -566,10 +572,10 @@ Section semantics.
         apply (H1 _ _ _ H2 H3).
   Qed.
 
-  Lemma teval_var_term_map_delete {σ m mv} x :
-    teval_var_term_map σ m mv → teval_var_term_map σ (delete x m) (delete x mv).
+  Lemma teval_vtmap_delete {σ m mv} x :
+    teval_vtmap σ m mv → teval_vtmap σ (delete x m) (delete x mv).
   Proof with auto.
-    intros []. unfold teval_var_term_map. split.
+    intros []. unfold teval_vtmap. split.
     - apply set_eq. intros. do 2 rewrite dom_delete. do 2 rewrite elem_of_difference.
       rewrite H...
     - intros. destruct (decide (x = x0)).
@@ -579,9 +585,9 @@ Section semantics.
         apply (H0 _ _ _ H1 H2).
   Qed.
 
-  Lemma teval_var_term_map_det {σ} m mv mv' :
-    teval_var_term_map σ m mv →
-    teval_var_term_map σ m mv' →
+  Lemma teval_vtmap_det {σ} m mv mv' :
+    teval_vtmap σ m mv →
+    teval_vtmap σ m mv' →
     mv = mv'.
   Proof with auto.
     intros. generalize dependent m. generalize dependent mv'.
@@ -603,20 +609,20 @@ Section semantics.
       assert (teval σ t v').
       { apply H2 with (x:=x); apply lookup_insert... }
       clear H1 H2. pose proof (teval_det _ _ _ H H4) as ->. clear H H4.
-      apply (teval_var_term_map_delete x) in Hmv, Hmv'.
+      apply (teval_vtmap_delete x) in Hmv, Hmv'.
       apply map_disjoint_singleton_l in H3, H0. rewrite (delete_insert) in Hmv, Hmv'...
       rewrite (delete_insert) in Hmv, Hmv'... rewrite (IH mv' m)...
   Qed.
 
-  Lemma teval_var_term_map_zip_cons_inv σ x xs t ts mv `{!OfSameLength xs ts} :
+  Lemma teval_vtmap_zip_cons_inv σ x xs t ts mv `{!OfSameLength xs ts} :
     NoDup (x :: xs) →
-    teval_var_term_map σ (to_var_term_map (x :: xs) (t :: ts)) mv →
+    teval_vtmap σ (to_vtmap (x :: xs) (t :: ts)) mv →
     ∃ v mv', teval σ t v ∧ mv = {[x := v]} ∪ mv' ∧ x ∉ dom mv'
-             ∧ teval_var_term_map σ (to_var_term_map xs ts) mv'.
+             ∧ teval_vtmap σ (to_vtmap xs ts) mv'.
   Proof with auto.
     intros. generalize dependent mv. generalize dependent t.
     generalize dependent x. induction_same_length xs ts as x' t'.
-    - unfold to_var_term_map in H1. simpl in H1.
+    - unfold to_vtmap in H1. simpl in H1.
       destruct H1 as []. rewrite insert_empty in H1. rewrite dom_singleton_L in H1.
       apply dom_singleton_inv_L in H1 as [v ->]. exists v, ∅. split_and!.
       + eapply H2; [apply lookup_insert|apply lookup_singleton].
@@ -625,25 +631,25 @@ Section semantics.
       + hnf. cbn. split... intros. apply lookup_empty_Some in H1 as [].
     - intros. apply NoDup_cons in H as []. assert (Hl:=H').
       apply of_same_length_rest in Hl. ospecialize (IH Hl x' _ t')...
-      destruct H0 as []. unfold to_var_term_map in H0. rewrite dom_list_to_map_zip_L in H0.
+      destruct H0 as []. unfold to_vtmap in H0. rewrite dom_list_to_map_zip_L in H0.
       2:{ typeclasses eauto. } rewrite list_to_set_cons in H0.
       apply dom_union_inv_L in H0 as (m1&m2&?&?&?&?).
       2: { set_solver. }
       apply dom_singleton_inv_L in H4 as [v Hv]. subst m1.
       rewrite <- insert_union_singleton_l in H0. subst mv. rename m2 into mv.
-      assert (teval_var_term_map σ (to_var_term_map (x' :: xs) (t' :: ts)) mv).
+      assert (teval_vtmap σ (to_vtmap (x' :: xs) (t' :: ts)) mv).
       { split.
-        - unfold to_var_term_map. rewrite dom_list_to_map_zip_L...
+        - unfold to_vtmap. rewrite dom_list_to_map_zip_L...
         - intros. assert (x0 ≠ x).
           { intros contra. subst. apply elem_of_dom_2 in H4. rewrite H5 in H4.
             apply elem_of_list_to_set in H4. contradiction. }
           apply (H2 x0)...
-          ++ unfold to_var_term_map. simpl. rewrite lookup_insert_ne...
+          ++ unfold to_vtmap. simpl. rewrite lookup_insert_ne...
           ++ rewrite lookup_insert_ne... }
       destruct (IH mv) as (v'&mv'&?&?&?&?)...
       exists v, mv. split_and!...
       + apply (H2 x).
-          * unfold to_var_term_map. simpl. rewrite lookup_insert...
+          * unfold to_vtmap. simpl. rewrite lookup_insert...
           * rewrite lookup_insert...
         + rewrite insert_union_singleton_l...
         + set_solver.
@@ -671,7 +677,7 @@ Section semantics.
   Qed.
 
   Lemma teval_msubst σ t0 m v0 mv :
-    teval_var_term_map σ m mv →
+    teval_vtmap σ m mv →
     teval σ (msubst_term t0 m) v0 ↔ teval (mv ∪ σ) t0 v0.
   Proof with auto.
     intros. generalize dependent v0. induction t0; intros.
@@ -703,7 +709,7 @@ Section semantics.
   Qed.
 
   Lemma afeval_msubst σ af m mv :
-    teval_var_term_map σ m mv →
+    teval_vtmap σ m mv →
     afeval σ (msubst_af af m) ↔ afeval (mv ∪ σ) af.
   Proof with auto.
     intros. destruct af...
@@ -727,7 +733,7 @@ Section semantics.
   Qed.
 
   Lemma feval_msubst σ A m mv :
-    teval_var_term_map σ m mv →
+    teval_vtmap σ m mv →
     feval σ (msubst A m) ↔ feval (mv ∪ σ) A.
   Proof with auto.
     intros. generalize dependent σ. induction A; intros σ Hteval; simp msubst; simp feval.
@@ -752,36 +758,36 @@ Section semantics.
 
   Global Instance msubst_proper : Proper((≡@{formula}) ==> (=) ==> (≡)) msubst.
   Proof with auto.
-    intros A B H m ? <- σ. destruct (teval_var_term_map_total σ m) as [mv ?].
+    intros A B H m ? <- σ. destruct (teval_vtmap_total σ m) as [mv ?].
     split; repeat rewrite feval_msubst with (mv:=mv); auto; intros; apply H...
   Qed.
 
   Global Instance msubst_proper_fent : Proper((⇛ₗ@{M}) ==> (=) ==> (⇛)) msubst.
   Proof with auto.
-    intros A B H m ? <- σ. destruct (teval_var_term_map_total σ m) as [mv ?].
+    intros A B H m ? <- σ. destruct (teval_vtmap_total σ m) as [mv ?].
     repeat rewrite feval_msubst with (mv:=mv); auto; intros; apply H...
   Qed.
 
   Lemma simpl_msubst_exists y A (xs : list variable) ts `{!OfSameLength xs ts} :
-    y ∉ (quant_msubst_fvars y A (to_var_term_map xs ts)) →
+    y ∉ (quant_msubst_fvars y A (to_vtmap xs ts)) →
     <! (∃ y, A)[[*xs \ *ts]] !> ≡ <! (∃ y, A [[*xs \ *ts]]) !>.
   Proof with auto.
     intros.
-    assert (fresh_var y (quant_msubst_fvars y A (to_var_term_map xs ts)) = y).
+    assert (fresh_var y (quant_msubst_fvars y A (to_vtmap xs ts)) = y).
     { apply fresh_var_id... }
     simp msubst. simpl. rewrite H0. rewrite fequiv_subst_diag...
   Qed.
 
   Lemma simpl_msubst_forall y A (xs : list variable) ts `{!OfSameLength xs ts} :
-    y ∉ (quant_msubst_fvars y A (to_var_term_map xs ts)) →
+    y ∉ (quant_msubst_fvars y A (to_vtmap xs ts)) →
     <! (∀ y, A)[[*xs \ *ts]] !> ≡ <! (∀ y, A [[*xs \ *ts]]) !>.
   Proof with auto.
     intros. unfold FForall. rewrite simpl_msubst_not. f_equiv.
     rewrite simpl_msubst_exists... rewrite simpl_msubst_not...
   Qed.
 
-  Local Lemma teval_var_term_map_total_inv σ mv :
-    ∃ m, teval_var_term_map σ m mv.
+  Local Lemma teval_vtmap_total_inv σ mv :
+    ∃ m, teval_vtmap σ m mv.
   Proof with auto.
     exists (TConst <$> mv). split.
     - rewrite dom_fmap_L...
@@ -789,31 +795,48 @@ Section semantics.
       constructor.
   Qed.
 
-  Lemma teval_delete_state_var_term_map_head σ t mv v :
+  Lemma teval_delete_state_vtmap_head σ t mv v :
     dom mv ## term_fvars t →
     teval (mv ∪ σ) t v ↔ teval σ t v.
   Proof with auto.
-    destruct (teval_var_term_map_total_inv σ mv) as [m Hm].
+    destruct (teval_vtmap_total_inv σ mv) as [m Hm].
     intros. rewrite <- teval_msubst with (m:=m)...
     rewrite msubst_term_id... rewrite <- (proj1 Hm)...
   Qed.
 
-  Lemma afeval_delete_state_var_term_map_head σ af mv :
+  Lemma afeval_delete_state_vtmap_head σ af mv :
     dom mv ## af_fvars af →
     afeval (mv ∪ σ) af ↔ afeval σ af.
   Proof with auto.
-    destruct (teval_var_term_map_total_inv σ mv) as [m Hm].
+    destruct (teval_vtmap_total_inv σ mv) as [m Hm].
     intros. rewrite <- afeval_msubst with (m:=m)...
     rewrite msubst_af_id... rewrite <- (proj1 Hm)...
   Qed.
 
-  Lemma feval_delete_state_var_term_map_head σ A mv :
+  Lemma feval_delete_state_vtmap_head σ A mv :
     dom mv ## formula_fvars A →
     feval (mv ∪ σ) A ↔ feval σ A.
   Proof with auto.
-    destruct (teval_var_term_map_total_inv σ mv) as [m Hm].
+    destruct (teval_vtmap_total_inv σ mv) as [m Hm].
     intros. rewrite <- feval_msubst with (m:=m)...
     rewrite msubst_id... rewrite <- (proj1 Hm)...
+  Qed.
+
+  Lemma teval_vtmap_delete_state_vtmap_head {σ1 m mv} (σ2 : gmap variable value)  :
+    dom σ2 ## vtmap_fvars m →
+    teval_vtmap (σ2 ∪ σ1) m mv ↔ teval_vtmap σ1 m mv.
+  Proof with auto.
+    intros. unfold teval_vtmap. split; intros []; split; auto; intros.
+    - unfold vtmap_fvars in H. set_unfold in H. setoid_rewrite elem_of_union_list in H.
+      setoid_rewrite elem_of_list_fmap in H. simpl in H. specialize (H1 _ _ _ H2 H3).
+      apply teval_delete_state_vtmap_head in H1... intros x' ??.
+      apply H in H5 as []. exists (term_fvars t). split... exists (x, t). simpl.
+      split... apply elem_of_map_to_list...
+    - unfold vtmap_fvars in H. set_unfold in H. setoid_rewrite elem_of_union_list in H.
+      setoid_rewrite elem_of_list_fmap in H. simpl in H. specialize (H1 _ _ _ H2 H3).
+      apply teval_delete_state_vtmap_head... intros x' ??.
+      apply H in H4 as []. exists (term_fvars t). split... exists (x, t). simpl.
+      split... apply elem_of_map_to_list...
   Qed.
 
   Lemma msubst_empty' A :
@@ -827,10 +850,10 @@ Section semantics.
     intros H σ. destruct (m !! x) eqn:E.
     2:{ rewrite delete_notin... }
     rewrite <- (insert_delete m x t) at 1...
-    pose proof (teval_var_term_map_total σ m) as [mv Hmv].
-    apply teval_var_term_map_delete with (x:=x) in Hmv as H1.
+    pose proof (teval_vtmap_total σ m) as [mv Hmv].
+    apply teval_vtmap_delete with (x:=x) in Hmv as H1.
     pose proof (teval_total σ t) as [v Hv].
-    apply (teval_var_term_map_insert x t v Hv) in H1 as H2.
+    apply (teval_vtmap_insert x t v Hv) in H1 as H2.
     rewrite feval_msubst with (mv:=(<[x:=v]> (delete x mv)))...
     rewrite feval_msubst with (mv:=(delete x mv))...
     rewrite <- (insert_union_l _ σ). rewrite feval_delete_state_var_head...
@@ -839,7 +862,7 @@ Section semantics.
   Lemma msubst_term_extract t0 x t m :
     m !! x = Some t →
     dom (delete x m) ## term_fvars t →
-    (x ∉ var_term_map_fvars (delete x m)) →
+    (x ∉ vtmap_fvars (delete x m)) →
     msubst_term t0 m = msubst_term (subst_term t0 x t) (delete x m).
   Proof with auto.
     induction t0; simpl; intros...
@@ -854,7 +877,7 @@ Section semantics.
   Lemma msubst_af_extract af x t m :
     m !! x = Some t →
     dom (delete x m) ## term_fvars t →
-    (x ∉ var_term_map_fvars (delete x m)) →
+    (x ∉ vtmap_fvars (delete x m)) →
     msubst_af af m = msubst_af (subst_af af x t) (delete x m).
   Proof with auto.
     destruct af; simpl; intros...
@@ -869,32 +892,32 @@ Section semantics.
   Proof with auto.
     intros. intros σ. rewrite <- (insert_delete m x t) at 1...
     pose proof (teval_total σ t) as [v Hv].
-    pose proof (teval_var_term_map_total σ (m)) as [mv Hmv].
-    apply teval_var_term_map_delete with (x:=x) in Hmv as H2.
-    apply (teval_var_term_map_insert x _ _ Hv) in H2 as H3.
+    pose proof (teval_vtmap_total σ (m)) as [mv Hmv].
+    apply teval_vtmap_delete with (x:=x) in Hmv as H2.
+    apply (teval_vtmap_insert x _ _ Hv) in H2 as H3.
     rewrite feval_msubst with (mv:=<[x:=v]> (delete x mv))...
     rewrite feval_msubst with (mv:=delete x mv)...
     assert (Hv':=Hv).
-    rewrite <- teval_delete_state_var_term_map_head with (mv:=delete x mv) in Hv'...
+    rewrite <- teval_delete_state_vtmap_head with (mv:=delete x mv) in Hv'...
     2: { rewrite (proj1 H2)... }
     rewrite feval_subst with (v:=v)... rewrite (insert_union_l (delete x mv))...
   Qed.
 
   Lemma msubst_extract_r' A x t m :
     m !! x = Some t →
-    (x ∉ var_term_map_fvars (delete x m)) →
+    (x ∉ vtmap_fvars (delete x m)) →
     msubst A m ≡ <! $(msubst A (delete x m)) [x \ t] !>.
   Proof with auto.
     intros. intros σ. rewrite <- (insert_delete m x t) at 1...
     pose proof (teval_total σ t) as [v Hv].
     rewrite feval_subst with (v:=v)...
-    pose proof (teval_var_term_map_total σ (m)) as [mv Hmv].
-    apply teval_var_term_map_delete with (x:=x) in Hmv as H2.
-    apply (teval_var_term_map_insert x _ _ Hv) in H2 as H3.
+    pose proof (teval_vtmap_total σ (m)) as [mv Hmv].
+    apply teval_vtmap_delete with (x:=x) in Hmv as H2.
+    apply (teval_vtmap_insert x _ _ Hv) in H2 as H3.
     rewrite feval_msubst with (mv:=<[x:=v]> (delete x mv))...
     rewrite feval_msubst with (mv:=delete x mv)...
     2:{ destruct H2 as []. split... intros. pose proof (H2 x0 t0 v0 H4 H5).
-        pose proof (not_elem_of_var_term_map_fvars _ _ H0). apply H7 in H4.
+        pose proof (not_elem_of_vtmap_fvars _ _ H0). apply H7 in H4.
         apply teval_delete_state_var_head... }
     rewrite <- (insert_union_r (delete x mv))...
     - rewrite <- (insert_union_l (delete x mv))...
@@ -904,7 +927,7 @@ Section semantics.
   Lemma msubst_subst_comm A x t m :
     m !! x = Some t →
     dom (delete x m) ## term_fvars t →
-    (x ∉ var_term_map_fvars (delete x m)) →
+    (x ∉ vtmap_fvars (delete x m)) →
     msubst (<! A[x \ t] !>) (delete x m) ≡ <! $(msubst A (delete x m)) [x \ t] !>.
   Proof with auto.
     intros. rewrite <- msubst_extract_l'... rewrite <- msubst_extract_r'...
@@ -912,12 +935,12 @@ Section semantics.
 
   Lemma msubst_empty A :
     <! A[[∅ \ ∅]] !> ≡ A.
-  Proof. unfold to_var_term_map. simpl. rewrite msubst_empty'. reflexivity. Qed.
+  Proof. unfold to_vtmap. simpl. rewrite msubst_empty'. reflexivity. Qed.
 
   Lemma msubst_single A x t :
     <! A[[x \ t]] !> ≡ <! A[x \ t] !>.
   Proof with auto.
-    unfold to_var_term_map. simpl. rewrite (msubst_extract_l' A x t _).
+    unfold to_vtmap. simpl. rewrite (msubst_extract_l' A x t _).
     - rewrite delete_insert... rewrite msubst_empty...
     - rewrite lookup_insert...
     - rewrite delete_insert... set_solver.
@@ -928,7 +951,7 @@ Section semantics.
     list_to_set xs ## term_fvars t →
     <! A[[x, *xs \ t, *ts]] !> ≡ <! A[x \ t][[*xs \ *ts]] !>.
   Proof with auto.
-    intros. unfold to_var_term_map. simpl. rewrite (msubst_extract_l' A x t).
+    intros. unfold to_vtmap. simpl. rewrite (msubst_extract_l' A x t).
     - rewrite delete_insert... apply lookup_list_to_map_zip_None...
     - rewrite lookup_insert...
     - rewrite dom_delete_L. rewrite dom_insert_L.
@@ -944,11 +967,11 @@ Section semantics.
     (x ∉ ⋃ (term_fvars <$> ts)) →
     <! A[[x, *xs \ t, *ts]] !> ≡ <! A[[*xs \ *ts]][x \ t] !>.
   Proof with auto.
-    intros. unfold to_var_term_map. repeat rewrite app_nil_r.
+    intros. unfold to_vtmap. repeat rewrite app_nil_r.
     simpl. rewrite (msubst_extract_r' A x t).
     - rewrite delete_insert... apply lookup_list_to_map_zip_None...
     - rewrite lookup_insert...
-    - intros contra. apply elem_of_var_term_map_fvars in contra as (y&t0&?&?).
+    - intros contra. apply elem_of_vtmap_fvars in contra as (y&t0&?&?).
       apply H0. apply elem_of_union_list. exists (term_fvars t0). split...
       rewrite delete_insert in H1...
       2:{ apply lookup_list_to_map_zip_None... }
@@ -984,7 +1007,7 @@ Section semantics.
     <! A[[*xs0, x, *xs1, x, *xs2 \ *ts0, t, *ts1, t, *ts2]] !> ≡
       <! A[[*xs0, x, *xs1, *xs2 \ *ts0, t, *ts1, *ts2]] !>.
   Proof with auto.
-    intros. unfold to_var_term_map. repeat rewrite app_nil_r. f_equiv.
+    intros. unfold to_vtmap. repeat rewrite app_nil_r. f_equiv.
     repeat rewrite zip_with_app... repeat rewrite list_to_map_app.
     simpl.
     rewrite (map_union_assoc (list_to_map (zip xs1 ts1))).
@@ -1000,7 +1023,7 @@ Section semantics.
     <! A[[*xs0, x, *xs1, x, *xs2 \ *ts0, t, *ts1, t, *ts2]] !> ≡
       <! A[[*xs0, *xs1, x, *xs2 \ *ts0, *ts1, t, *ts2]] !>.
   Proof with auto.
-    intros. unfold to_var_term_map. repeat rewrite app_nil_r. f_equiv.
+    intros. unfold to_vtmap. repeat rewrite app_nil_r. f_equiv.
     repeat rewrite zip_with_app... repeat rewrite list_to_map_app.
     simpl.
     rewrite (map_union_assoc (list_to_map (zip xs1 ts1))).
@@ -1018,12 +1041,12 @@ Section semantics.
     x1 ≠ x2 →
     x1 ∉ xs1 →
     x2 ∉ xs1 →
-    msubst A (@to_var_term_map _ (xs0 ++ [x1] ++ xs1 ++ [x2] ++ xs2)
+    msubst A (@to_vtmap _ (xs0 ++ [x1] ++ xs1 ++ [x2] ++ xs2)
                 (ts0 ++ [t1] ++ ts1 ++ [t2] ++ ts2) Hl1) ≡
-    msubst A (@to_var_term_map _ (xs0 ++ [x2] ++ xs1 ++ [x1] ++ xs2)
+    msubst A (@to_vtmap _ (xs0 ++ [x2] ++ xs1 ++ [x1] ++ xs2)
                 (ts0 ++ [t2] ++ ts1 ++ [t1] ++ ts2) Hl2).
   Proof with auto.
-    intros. unfold to_var_term_map.
+    intros. unfold to_vtmap.
     pose proof (@of_same_length _ _ _ _ Hl1).
     repeat rewrite length_app in H2. simpl in H2.
     repeat rewrite app_nil_r. f_equiv.
@@ -1050,9 +1073,9 @@ Section semantics.
       `{!OfSameLength xs0 ts0} `{!OfSameLength xs1 ts1}
       {Hl1 Hl2} :
     x1 ≠ x2 →
-    msubst A (@to_var_term_map _ (xs0 ++ [x1] ++ [x2] ++ xs1)
+    msubst A (@to_vtmap _ (xs0 ++ [x1] ++ [x2] ++ xs1)
                 (ts0 ++ [t1] ++ [t2] ++ ts1) Hl1) ≡
-    msubst A (@to_var_term_map _ (xs0 ++ [x2] ++ [x1] ++ xs1)
+    msubst A (@to_vtmap _ (xs0 ++ [x2] ++ [x1] ++ xs1)
                 (ts0 ++ [t2] ++ [t1] ++ ts1) Hl2).
   Proof with auto.
     intros.
@@ -1071,8 +1094,8 @@ Section semantics.
     - rewrite IHA...
     - rewrite IHA1; [| set_solver]. rewrite IHA2; [| set_solver]...
     - rewrite IHA1; [| set_solver]. rewrite IHA2; [| set_solver]...
-    - simpl. generalize_fresh_var_for_msubst x A (to_var_term_map xs ts) as x'.
-      unfold to_var_term_map in H4. rewrite dom_list_to_map_zip_L in H4...
+    - simpl. generalize_fresh_var_for_msubst x A (to_vtmap xs ts) as x'.
+      unfold to_vtmap in H4. rewrite dom_list_to_map_zip_L in H4...
       destruct H3.
       + subst. f_equiv. rewrite H0...
         * rewrite fequiv_subst_diag...
@@ -1092,11 +1115,11 @@ Section semantics.
     <! A [[*xs1 \ ⇑ₓ₊ xs2]] [[*xs2 \ *ts]] !> ≡ <! A[[*xs1 \ *ts]] !>.
   Proof with auto.
     intros ? Hnodup ?. intros σ.
-    opose proof (teval_var_term_map_total σ (to_var_term_map xs1 ts)) as [mv ?].
-    opose proof (teval_var_term_map_total σ _) as [mvx2t ?].
+    opose proof (teval_vtmap_total σ (to_vtmap xs1 ts)) as [mv ?].
+    opose proof (teval_vtmap_total σ _) as [mvx2t ?].
     rewrite feval_msubst with (mv:=mvx2t) by exact H2.
     rewrite feval_msubst with (mv:=mv).
-    2:{ unfold to_var_term_map in *. destruct H1 as [], H2 as [].
+    2:{ unfold to_vtmap in *. destruct H1 as [], H2 as [].
         split.
         - rewrite dom_list_to_map_zip_L in *... typeclasses eauto.
         - intros x1 tx2 v ??. apply lookup_list_to_map_zip_Some in H5 as (i&?&?&?)...
@@ -1119,13 +1142,88 @@ Section semantics.
           constructor. apply (lookup_total_union_l' _ σ)... }
     rewrite map_union_assoc. rewrite (map_union_comm mv).
     2:{ destruct H1 as (?&?), H2 as (?&?). apply map_disjoint_dom. rewrite H1.
-        rewrite H2. unfold to_var_term_map. rewrite dom_list_to_map_zip_L...
+        rewrite H2. unfold to_vtmap. rewrite dom_list_to_map_zip_L...
         rewrite dom_list_to_map_zip_L...
         set_solver. }
-    rewrite <- map_union_assoc. rewrite feval_delete_state_var_term_map_head.
-    2:{ unfold teval_var_term_map in H2. destruct H2 as [-> _]. unfold to_var_term_map.
+    rewrite <- map_union_assoc. rewrite feval_delete_state_vtmap_head.
+    2:{ unfold teval_vtmap in H2. destruct H2 as [-> _]. unfold to_vtmap.
         rewrite dom_list_to_map_zip_L... }
     rewrite feval_msubst with (mv:=mv)...
+  Qed.
+
+  Lemma msubst_term_msubst_term_eq t xs ts1 ts2 `{!OfSameLength xs ts1} `{!OfSameLength xs ts2} :
+    NoDup xs →
+    <! t [[ₜ *xs \ *ts1 ]][[ₜ *xs \ *ts2 ]] !> ≡
+      <! t [[ₜ *xs \ *$((λ t, <! t[[ₜ *xs \ *ts2]] !>) <$> ts1)]] !>.
+  Proof with auto.
+    intros Hnodup σ v.
+    opose proof (teval_vtmap_total σ _) as [mv1 ?].
+    rewrite teval_msubst with (mv:=mv1) by exact H.
+    opose proof (teval_vtmap_total _ _) as [mv2 ?].
+    rewrite teval_msubst with (mv:=mv2) by exact H0.
+    opose proof (teval_vtmap_total _ _) as [mv3 ?].
+    rewrite teval_msubst with (mv:=mv3) by exact H1.
+    rewrite map_union_assoc. f_equiv. f_equiv. apply (map_eq _ mv3).
+    intros x. destruct H as [], H0 as [], H1 as [].
+    destruct (decide (x ∈ xs)).
+    2:{ enough (x ∉ dom mv3 ∧ x ∉ dom (mv2 ∪ mv1)).
+        - destruct H5. apply not_elem_of_dom in H5, H6. rewrite H5, H6...
+        - rewrite dom_union. rewrite H, H0, H1. unfold to_vtmap.
+          rewrite dom_list_to_map_zip_L; [|apply of_same_length_fmap_r].
+          rewrite dom_list_to_map_zip_L; [|auto]. rewrite dom_list_to_map_zip_L; [|auto].
+          rewrite union_idemp_L. split; set_solver. }
+    assert (is_Some (mv2 !! x)).
+    { apply elem_of_dom. rewrite H0. unfold to_vtmap. rewrite dom_list_to_map_zip_L...
+      set_solver. }
+    rewrite lookup_union_l'... destruct H5 as [v2 ?].
+    assert (is_Some (mv3 !! x)) as (v3&?).
+    { apply elem_of_dom. rewrite H1. unfold to_vtmap. rewrite dom_list_to_map_zip_L;
+        [set_solver|]. apply of_same_length_fmap_r. }
+    rewrite H5, H6. f_equal. apply elem_of_list_lookup in e as (i&?).
+    destruct (lookup_of_same_length_l ts1 H7) as (t1&?).
+    eapply (@teval_det _ (mv1 ∪ σ)) with (t:=t1).
+    - apply H3 with (x:=x)... unfold to_vtmap. apply lookup_list_to_map_zip_Some...
+      exists i. split_and!... intros. eapply NoDup_lookup with (i:=i) in H9... lia.
+    - specialize (H4 x <! t1 [[ₜ *xs \ *ts2]] !> v3).
+      rewrite <- teval_msubst; [apply H4| split; auto]... unfold to_vtmap.
+      apply lookup_list_to_map_zip_Some.
+      { apply of_same_length_fmap_r. }
+      exists i. split_and!...
+      + apply list_lookup_fmap_Some. exists t1. split...
+      + intros. apply NoDup_lookup with (i:=i) in H9... lia.
+  Qed.
+
+  Lemma msubst_term_msubst_term_eq_cancel t xs ts1 ts2
+    `{!OfSameLength xs ts1} `{!OfSameLength xs ts2} :
+    list_to_set xs ## ⋃ (term_fvars <$> ts1) →
+    NoDup xs →
+    <! t [[ₜ *xs \ *ts1 ]][[ₜ *xs \ *ts2 ]] !> ≡
+      <! t [[ₜ *xs \ *ts1 ]] !>.
+  Proof with auto.
+    intros. rewrite msubst_term_msubst_term_eq... f_equiv. apply map_eq. intros x.
+    unfold to_vtmap.
+    destruct
+      (list_to_map (zip xs ((λ t0, msubst_term t0 (list_to_map (zip xs ts2))) <$> ts1)) !! x)
+        as [t2|]
+        eqn:E1;
+      destruct (list_to_map (zip xs ts1) !! x) as [t1|] eqn:E2...
+      - apply lookup_list_to_map_zip_Some in E2 as (i&?&?&_)...
+        assert (H3:=H1). apply (lookup_of_same_length_l ts2) in H3 as [t2' ?].
+        apply lookup_list_to_map_zip_Some in E1 as (j&?&?&_)...
+        2:{ typeclasses eauto. }
+        apply list_lookup_fmap_Some in H5 as (t1'&?&?).
+        apply NoDup_lookup with (j:=j) in H1... subst j. rewrite H5 in H2. inversion H2.
+        subst t1'. subst t2. f_equal. fold (to_vtmap xs ts2). rewrite msubst_term_non_free...
+        clear dependent x. intros x ??. apply (H x)... apply elem_of_union_list.
+        exists (term_fvars t1). split... apply elem_of_list_fmap. exists t1. split...
+        apply elem_of_list_lookup_2 in H5...
+      - apply lookup_list_to_map_zip_Some in E1 as (?&?&_)...
+        2:{ typeclasses eauto. }
+        apply lookup_list_to_map_zip_None in E2... apply elem_of_list_lookup_2 in H1. done.
+      - apply lookup_list_to_map_zip_Some in E2 as (?&?&_)...
+        apply lookup_list_to_map_zip_None in E1...
+        2:{ typeclasses eauto. }
+        apply elem_of_list_lookup_2 in H1. done.
   Qed.
 
   Lemma msubst_msubst_eq A xs ts1 ts2 `{!OfSameLength xs ts1} `{!OfSameLength xs ts2} :
@@ -1133,41 +1231,42 @@ Section semantics.
     <! A [[*xs \ *ts1]][[*xs \ *ts2]] !> ≡ <! A [[*xs \ *$((λ t, <! t[[ₜ *xs \ *ts2]] !>) <$> ts1)]] !>.
   Proof with auto.
     intros Hnodup σ.
-    opose proof (teval_var_term_map_total σ _) as [mv1 ?].
+    opose proof (teval_vtmap_total σ _) as [mv1 ?].
     rewrite feval_msubst with (mv:=mv1) by exact H.
-    opose proof (teval_var_term_map_total _ _) as [mv2 ?].
+    opose proof (teval_vtmap_total _ _) as [mv2 ?].
     rewrite feval_msubst with (mv:=mv2) by exact H0.
-    opose proof (teval_var_term_map_total _ _) as [mv3 ?].
+    opose proof (teval_vtmap_total _ _) as [mv3 ?].
     rewrite feval_msubst with (mv:=mv3) by exact H1.
     rewrite map_union_assoc. f_equiv. f_equiv. apply (map_eq _ mv3).
     intros x. destruct H as [], H0 as [], H1 as [].
     destruct (decide (x ∈ xs)).
     2:{ enough (x ∉ dom mv3 ∧ x ∉ dom (mv2 ∪ mv1)).
         - destruct H5. apply not_elem_of_dom in H5, H6. rewrite H5, H6...
-        - rewrite dom_union. rewrite H, H0, H1. unfold to_var_term_map.
+        - rewrite dom_union. rewrite H, H0, H1. unfold to_vtmap.
           rewrite dom_list_to_map_zip_L; [|apply of_same_length_fmap_r].
           rewrite dom_list_to_map_zip_L; [|auto]. rewrite dom_list_to_map_zip_L; [|auto].
           rewrite union_idemp_L. split; set_solver. }
     assert (is_Some (mv2 !! x)).
-    { apply elem_of_dom. rewrite H0. unfold to_var_term_map. rewrite dom_list_to_map_zip_L...
+    { apply elem_of_dom. rewrite H0. unfold to_vtmap. rewrite dom_list_to_map_zip_L...
       set_solver. }
     rewrite lookup_union_l'... destruct H5 as [v2 ?].
     assert (is_Some (mv3 !! x)) as (v3&?).
-    { apply elem_of_dom. rewrite H1. unfold to_var_term_map. rewrite dom_list_to_map_zip_L;
+    { apply elem_of_dom. rewrite H1. unfold to_vtmap. rewrite dom_list_to_map_zip_L;
         [set_solver|]. apply of_same_length_fmap_r. }
     rewrite H5, H6. f_equal. apply elem_of_list_lookup in e as (i&?).
     destruct (lookup_of_same_length_l ts1 H7) as (t1&?).
     eapply (@teval_det _ (mv1 ∪ σ)) with (t:=t1).
-    - apply H3 with (x:=x)... unfold to_var_term_map. apply lookup_list_to_map_zip_Some...
+    - apply H3 with (x:=x)... unfold to_vtmap. apply lookup_list_to_map_zip_Some...
       exists i. split_and!... intros. eapply NoDup_lookup with (i:=i) in H9... lia.
     - specialize (H4 x <! t1 [[ₜ *xs \ *ts2]] !> v3).
-      rewrite <- teval_msubst; [apply H4| split; auto]... unfold to_var_term_map.
+      rewrite <- teval_msubst; [apply H4| split; auto]... unfold to_vtmap.
       apply lookup_list_to_map_zip_Some.
       { apply of_same_length_fmap_r. }
       exists i. split_and!...
       + apply list_lookup_fmap_Some. exists t1. split...
       + intros. apply NoDup_lookup with (i:=i) in H9... lia.
   Qed.
+
 
   (* TODO: move it *)
   Lemma fsubst_fsubst_ne A x1 t1 x2 t2 :
@@ -1198,6 +1297,85 @@ Section semantics.
       + rewrite <- teval_delete_state_var_head; [exact H3|]...
   Qed.
 
+  Lemma msubst_term_msubst_term_disj t xs1 ts1 xs2 ts2 `{!OfSameLength xs1 ts1} `{!OfSameLength xs2 ts2} :
+    xs1 ## xs2 →
+    NoDup xs1 →
+    NoDup xs2 →
+    list_to_set xs1 ## ⋃ (term_fvars <$> ts2) →
+    <! t [[ₜ *xs1 \ *ts1 ]][[ₜ *xs2 \ *ts2 ]] !> ≡
+      <! t [[ₜ *xs2 \ *ts2 ]] [[ₜ *xs1 \ *$((λ t, <! t[[ₜ *xs2 \ *ts2]] !>) <$> ts1) ]] !>.
+  Proof with auto.
+    intros Hdisjoint Hnodup1 Hnodup2 Hfree σ v.
+    opose proof (teval_vtmap_total σ _) as [mv1 ?].
+    rewrite teval_msubst with (mv:=mv1) by exact H.
+    opose proof (teval_vtmap_total _ _) as [mv2 ?].
+    rewrite teval_msubst with (mv:=mv2) by exact H0.
+    opose proof (teval_vtmap_total _ _) as [mv3 ?].
+    rewrite teval_msubst with (mv:=mv3) by exact H1.
+    opose proof (teval_vtmap_total _ _) as [mv4 ?].
+    rewrite teval_msubst with (mv:=mv4) by exact H2.
+    rewrite map_union_assoc. rewrite map_union_assoc.
+    f_equiv. f_equiv. apply (map_eq (mv2 ∪ mv1)).
+    intros x. destruct H as [], H0 as [], H1 as [], H2 as [].
+    destruct (decide (x ∈ xs1 ∨ x ∈ xs2)).
+    2:{ apply Decidable.not_or in n as []. enough (x ∉ dom (mv2 ∪ mv1) ∧ x ∉ dom (mv4 ∪ mv3)).
+        - destruct H9. apply not_elem_of_dom in H9, H10. rewrite H9, H10...
+        - do 2 rewrite dom_union. rewrite H, H0, H1, H2. unfold to_vtmap.
+          rewrite dom_list_to_map_zip_L... rewrite dom_list_to_map_zip_L...
+          rewrite dom_list_to_map_zip_L; [|apply of_same_length_fmap_r].
+          clear dependent mv1 mv2 mv3 mv4. split; set_solver. }
+    destruct o.
+    - apply Hdisjoint in H7 as ?.
+      assert (is_Some (mv2 !! x)).
+      { apply elem_of_dom. rewrite H0. unfold to_vtmap. rewrite dom_list_to_map_zip_L...
+        clear dependent mv1 mv2 mv3 mv4. set_solver. }
+      assert (is_Some (mv3 !! x)).
+      { apply elem_of_dom. rewrite H1. unfold to_vtmap. clear dependent mv1 mv2 mv3 mv4.
+        rewrite dom_list_to_map_zip_L; [set_solver|]. typeclasses eauto. }
+      assert (mv4 !! x = None).
+      { apply not_elem_of_dom. rewrite H2. unfold to_vtmap. clear dependent mv1 mv2 mv3 mv4.
+        rewrite dom_list_to_map_zip_L; [set_solver|]... }
+      rewrite lookup_union_l'... rewrite lookup_union_r... destruct H9 as [v2 ?].
+      destruct H10 as [v3 ?]. apply elem_of_list_lookup in H7 as (i&?).
+      destruct (lookup_of_same_length_l ts1 H7) as (t'&?). rewrite H9, H10. f_equal.
+      eapply (@teval_det _ (mv1 ∪ σ)) with (t:=t').
+      + apply H4 with (x:=x)... unfold to_vtmap. apply lookup_list_to_map_zip_Some...
+        exists i. split_and!... intros. eapply NoDup_lookup with (i:=i) in H13... lia.
+      + specialize (H5 x <! t' [[ₜ *xs2 \ *ts2 ]] !> v3).
+        rewrite <- teval_msubst; [apply H5| split; auto]... unfold to_vtmap.
+        apply lookup_list_to_map_zip_Some.
+        { apply of_same_length_fmap_r. }
+        exists i. split_and!...
+        * apply list_lookup_fmap_Some. exists t'. split...
+        * intros. apply NoDup_lookup with (i:=i) in H13... lia.
+    - assert (x ∉ xs1) by (intros contra; apply (Hdisjoint x); auto).
+      assert (is_Some (mv1 !! x)).
+      { apply elem_of_dom. rewrite H. unfold to_vtmap. rewrite dom_list_to_map_zip_L...
+        clear dependent mv1 mv2 mv3 mv4. set_solver. }
+      assert (is_Some (mv4 !! x)).
+      { apply elem_of_dom. rewrite H2. unfold to_vtmap. clear dependent mv1 mv2 mv3 mv4.
+        rewrite dom_list_to_map_zip_L; [set_solver|]. typeclasses eauto. }
+      assert (mv2 !! x = None).
+      { apply not_elem_of_dom. rewrite H0. unfold to_vtmap. clear dependent mv1 mv2 mv3 mv4.
+        rewrite dom_list_to_map_zip_L; [set_solver|]... }
+      rewrite lookup_union_r... destruct H9 as [v1 ?].
+      rewrite lookup_union_l'... destruct H10 as [v4 ?].
+      apply elem_of_list_lookup in H7 as (i&?).
+      destruct (lookup_of_same_length_l ts2 H7) as (t'&?). rewrite H9, H10. f_equal.
+      eapply (@teval_det _ σ) with (t:=t').
+      + apply H3 with (x:=x)... unfold to_vtmap. apply lookup_list_to_map_zip_Some...
+        exists i. split_and!... intros. apply NoDup_lookup with (i:=i) in H13... lia.
+      + ospecialize (H6 x t' v4 _ _)...
+        { unfold to_vtmap. apply lookup_list_to_map_zip_Some... exists i. split_and!...
+          intros. apply NoDup_lookup with (i:=i) in H13... lia. }
+        rewrite <- teval_delete_state_vtmap_head; [exact H6|].
+        rewrite H1. unfold to_vtmap. rewrite dom_list_to_map_zip_L.
+        2:{ typeclasses eauto. }
+        clear dependent mv1 mv2 mv3 mv4 x. intros x ??. apply Hfree in H.
+        apply H. apply elem_of_union_list. apply elem_of_list_lookup_2 in H12.
+        set_solver.
+  Qed.
+
   Lemma msubst_msubst_disj A xs1 ts1 xs2 ts2 `{!OfSameLength xs1 ts1} `{!OfSameLength xs2 ts2} :
     xs1 ## xs2 →
     NoDup xs1 →
@@ -1206,13 +1384,13 @@ Section semantics.
     <! A [[*xs1 \ *ts1]][[*xs2 \ *ts2]] !> ≡ <! A [[*xs2 \ *ts2]] [[*xs1 \ *$((λ t, <! t[[ₜ *xs2 \ *ts2]] !>) <$> ts1)]] !>.
   Proof with auto.
     intros Hdisjoint Hnodup1 Hnodup2 Hfree σ.
-    opose proof (teval_var_term_map_total σ _) as [mv1 ?].
+    opose proof (teval_vtmap_total σ _) as [mv1 ?].
     rewrite feval_msubst with (mv:=mv1) by exact H.
-    opose proof (teval_var_term_map_total _ _) as [mv2 ?].
+    opose proof (teval_vtmap_total _ _) as [mv2 ?].
     rewrite feval_msubst with (mv:=mv2) by exact H0.
-    opose proof (teval_var_term_map_total _ _) as [mv3 ?].
+    opose proof (teval_vtmap_total _ _) as [mv3 ?].
     rewrite feval_msubst with (mv:=mv3) by exact H1.
-    opose proof (teval_var_term_map_total _ _) as [mv4 ?].
+    opose proof (teval_vtmap_total _ _) as [mv4 ?].
     rewrite feval_msubst with (mv:=mv4) by exact H2.
     rewrite map_union_assoc. rewrite map_union_assoc.
     f_equiv. f_equiv. apply (map_eq (mv2 ∪ mv1)).
@@ -1220,29 +1398,29 @@ Section semantics.
     destruct (decide (x ∈ xs1 ∨ x ∈ xs2)).
     2:{ apply Decidable.not_or in n as []. enough (x ∉ dom (mv2 ∪ mv1) ∧ x ∉ dom (mv4 ∪ mv3)).
         - destruct H9. apply not_elem_of_dom in H9, H10. rewrite H9, H10...
-        - do 2 rewrite dom_union. rewrite H, H0, H1, H2. unfold to_var_term_map.
+        - do 2 rewrite dom_union. rewrite H, H0, H1, H2. unfold to_vtmap.
           rewrite dom_list_to_map_zip_L... rewrite dom_list_to_map_zip_L...
           rewrite dom_list_to_map_zip_L; [|apply of_same_length_fmap_r].
           clear dependent mv1 mv2 mv3 mv4. split; set_solver. }
     destruct o.
     - apply Hdisjoint in H7 as ?.
       assert (is_Some (mv2 !! x)).
-      { apply elem_of_dom. rewrite H0. unfold to_var_term_map. rewrite dom_list_to_map_zip_L...
+      { apply elem_of_dom. rewrite H0. unfold to_vtmap. rewrite dom_list_to_map_zip_L...
         clear dependent mv1 mv2 mv3 mv4. set_solver. }
       assert (is_Some (mv3 !! x)).
-      { apply elem_of_dom. rewrite H1. unfold to_var_term_map. clear dependent mv1 mv2 mv3 mv4.
+      { apply elem_of_dom. rewrite H1. unfold to_vtmap. clear dependent mv1 mv2 mv3 mv4.
         rewrite dom_list_to_map_zip_L; [set_solver|]. typeclasses eauto. }
       assert (mv4 !! x = None).
-      { apply not_elem_of_dom. rewrite H2. unfold to_var_term_map. clear dependent mv1 mv2 mv3 mv4.
+      { apply not_elem_of_dom. rewrite H2. unfold to_vtmap. clear dependent mv1 mv2 mv3 mv4.
         rewrite dom_list_to_map_zip_L; [set_solver|]... }
       rewrite lookup_union_l'... rewrite lookup_union_r... destruct H9 as [v2 ?].
       destruct H10 as [v3 ?]. apply elem_of_list_lookup in H7 as (i&?).
       destruct (lookup_of_same_length_l ts1 H7) as (t&?). rewrite H9, H10. f_equal.
       eapply (@teval_det _ (mv1 ∪ σ)) with (t:=t).
-      + apply H4 with (x:=x)... unfold to_var_term_map. apply lookup_list_to_map_zip_Some...
+      + apply H4 with (x:=x)... unfold to_vtmap. apply lookup_list_to_map_zip_Some...
         exists i. split_and!... intros. eapply NoDup_lookup with (i:=i) in H13... lia.
       + specialize (H5 x <! t [[ₜ *xs2 \ *ts2 ]] !> v3).
-        rewrite <- teval_msubst; [apply H5| split; auto]... unfold to_var_term_map.
+        rewrite <- teval_msubst; [apply H5| split; auto]... unfold to_vtmap.
         apply lookup_list_to_map_zip_Some.
         { apply of_same_length_fmap_r. }
         exists i. split_and!...
@@ -1250,26 +1428,26 @@ Section semantics.
         * intros. apply NoDup_lookup with (i:=i) in H13... lia.
     - assert (x ∉ xs1) by (intros contra; apply (Hdisjoint x); auto).
       assert (is_Some (mv1 !! x)).
-      { apply elem_of_dom. rewrite H. unfold to_var_term_map. rewrite dom_list_to_map_zip_L...
+      { apply elem_of_dom. rewrite H. unfold to_vtmap. rewrite dom_list_to_map_zip_L...
         clear dependent mv1 mv2 mv3 mv4. set_solver. }
       assert (is_Some (mv4 !! x)).
-      { apply elem_of_dom. rewrite H2. unfold to_var_term_map. clear dependent mv1 mv2 mv3 mv4.
+      { apply elem_of_dom. rewrite H2. unfold to_vtmap. clear dependent mv1 mv2 mv3 mv4.
         rewrite dom_list_to_map_zip_L; [set_solver|]. typeclasses eauto. }
       assert (mv2 !! x = None).
-      { apply not_elem_of_dom. rewrite H0. unfold to_var_term_map. clear dependent mv1 mv2 mv3 mv4.
+      { apply not_elem_of_dom. rewrite H0. unfold to_vtmap. clear dependent mv1 mv2 mv3 mv4.
         rewrite dom_list_to_map_zip_L; [set_solver|]... }
       rewrite lookup_union_r... destruct H9 as [v1 ?].
       rewrite lookup_union_l'... destruct H10 as [v4 ?].
       apply elem_of_list_lookup in H7 as (i&?).
       destruct (lookup_of_same_length_l ts2 H7) as (t&?). rewrite H9, H10. f_equal.
       eapply (@teval_det _ σ) with (t:=t).
-      + apply H3 with (x:=x)... unfold to_var_term_map. apply lookup_list_to_map_zip_Some...
+      + apply H3 with (x:=x)... unfold to_vtmap. apply lookup_list_to_map_zip_Some...
         exists i. split_and!... intros. apply NoDup_lookup with (i:=i) in H13... lia.
       + ospecialize (H6 x t v4 _ _)...
-        { unfold to_var_term_map. apply lookup_list_to_map_zip_Some... exists i. split_and!...
+        { unfold to_vtmap. apply lookup_list_to_map_zip_Some... exists i. split_and!...
           intros. apply NoDup_lookup with (i:=i) in H13... lia. }
-        rewrite <- teval_delete_state_var_term_map_head; [exact H6|].
-        rewrite H1. unfold to_var_term_map. rewrite dom_list_to_map_zip_L.
+        rewrite <- teval_delete_state_vtmap_head; [exact H6|].
+        rewrite H1. unfold to_vtmap. rewrite dom_list_to_map_zip_L.
         2:{ typeclasses eauto. }
         clear dependent mv1 mv2 mv3 mv4 x. intros x ??. apply Hfree in H.
         apply H. apply elem_of_union_list. apply elem_of_list_lookup_2 in H12.
@@ -1280,7 +1458,7 @@ Section semantics.
     NoDup xs →
     NoDup xs' →
     (xs, ts) ≡ₚₚ (xs', ts') →
-    msubst A (to_var_term_map xs ts) ≡ msubst A (to_var_term_map xs' ts').
+    msubst A (to_vtmap xs ts) ≡ msubst A (to_vtmap xs' ts').
   Proof with auto.
     intros. f_equiv. apply zip_pair_Permutation_list_to_map_zip... typeclasses eauto.
   Qed.
