src/Examples/Common.v
@@ -1,0 +1,18 @@
+From Stdlib Require Import Strings.String.
+From MRC Require Import RefCalc.
+
+Definition x := Model.raw_var "x".
+Definition y := Model.raw_var "y".
+Definition z := Model.raw_var "z".
+Definition t := Model.raw_var "t".
+Definition i := Model.raw_var "i".
+Definition j := Model.raw_var "j".
+Definition k := Model.raw_var "k".
+
+Definition x₀ := Model.to_initial_var x.
+Definition y₀ := Model.to_initial_var y.
+Definition z₀ := Model.to_initial_var z.
+Definition t₀ := Model.to_initial_var t.
+Definition i₀ := Model.to_initial_var i.
+Definition j₀ := Model.to_initial_var j.
+Definition k₀ := Model.to_initial_var k.
